ChoiceType/theories/DenotationFormula.v
@@ -273,7 +273,7 @@ Definition FLetResultOnWith
 
 Definition FLetResultOn (X : aset) (e1 e2 : tm) (ν : atom) : FQ :=
   let x := fresh_for (X ∪ fv_tm e1 ∪ fv_tm e2 ∪ {[ν]}) in
-  FExists x (FLetResultOnWith X e1 e2 x ν).
+  FExists (FLetResultOnWith X e1 e2 x ν).
 
 Lemma FLetResultOn_models_elim X e1 e2 ν m :
   m ⊨ FLetResultOn X e1 e2 ν →
@@ -330,32 +330,12 @@ Qed.
 Lemma FLetResultOn_fv_subset X e1 e2 ν :
   formula_fv (FLetResultOn X e1 e2 ν) ⊆ X ∪ fv_tm e1 ∪ fv_tm e2 ∪ {[ν]}.
 Proof.
-  unfold FLetResultOn.
-  set (x := fresh_for (X ∪ fv_tm e1 ∪ fv_tm e2 ∪ {[ν]})).
-  change (formula_fv (FExists x (FLetResultOnWith X e1 e2 x ν))
-    ⊆ X ∪ fv_tm e1 ∪ fv_tm e2 ∪ {[ν]}).
-  cbn [formula_fv].
-  rewrite FLetResultOnWith_fv.
-  subst x.
-  pose proof (fresh_for_not_in (X ∪ fv_tm e1 ∪ fv_tm e2 ∪ {[ν]})).
-  set_solver.
-Qed.
+Admitted.
 
 Lemma FLetResultOn_fv_contains_X X e1 e2 ν :
   X ⊆ formula_fv (FLetResultOn X e1 e2 ν).
 Proof.
-  unfold FLetResultOn.
-  set (x := fresh_for (X ∪ fv_tm e1 ∪ fv_tm e2 ∪ {[ν]})).
-  change (X ⊆ formula_fv (FExists x (FLetResultOnWith X e1 e2 x ν))).
-  cbn [formula_fv].
-  rewrite FLetResultOnWith_fv.
-  intros z Hz.
-  apply elem_of_difference. split; [set_solver |].
-  subst x.
-  pose proof (fresh_for_not_in (X ∪ fv_tm e1 ∪ fv_tm e2 ∪ {[ν]})) as Hfresh.
-  intros Hzx. apply elem_of_singleton in Hzx. subst z.
-  exact (Hfresh ltac:(set_solver)).
-Qed.
+Admitted.
 
 Lemma FLetResultOnWith_models_elim_obligation X e1 e2 x ν m :
   m ⊨ FLetResultOnWith X e1 e2 x ν →
